src/Dafny/examples/simple.i.dfy
@@ -17,9 +17,9 @@ lemma lvm_lemma_Empty_Test(lvm_b0:lvm_codes, lvm_s0:lvm_state, lvm_sN:lvm_state,
   requires lvm_is_src_opr(src, lvm_s0)
   requires lvm_get_ok(lvm_s0)
   ensures  lvm_ensure(lvm_b0, lvm_bM, lvm_s0, lvm_sM, lvm_sN,o)
-  ensures  lvm_get_ok(lvm_sM)
+  ensures  lvm_get_ok(lvm_sM) // ValidState(sM)
   ensures  lvm_state_eq(lvm_sM, lvm_s0)
-ensures lvm_state_eq(lvm_sM, lvm_update_mem( lvm_sM, lvm_update_ok(lvm_sM, lvm_sM)))
+  ensures  lvm_state_eq(lvm_sM, lvm_update_mem( lvm_sM, lvm_update_ok(lvm_sM, lvm_sM)))
 {
   reveal_lvm_code_Empty_Test();
   reveal_eval_code();
@@ -35,14 +35,11 @@ ensures lvm_state_eq(lvm_sM, lvm_update_mem( lvm_sM, lvm_update_ok(lvm_sM, lvm_s
   assert evalBlock(lvm_get_block(lvm_b0.hd),lvm_s0, lvm_s0,o);
   assert forall r :: r == lvm_s0 ==> eval_code(lvm_b0.hd,lvm_s0,r,o);
   assert evalCode_lax(Block(lvm_b0), lvm_s0, lvm_sN, o);
-//   assert exists r' :: evalBlock(lvm_b0.tl, lvm_s0, r',o);
-// assert Block(CNil).CNil?;
-assert evalBlock(lvm_b0, lvm_s0, lvm_sN,o) ==> exists r' :: evalCode(lvm_b0.hd, lvm_s0, r',o) && evalBlock(lvm_b0.tl, r', lvm_sN,o);
-assert exists r' :: if evalCode(lvm_b0.hd, lvm_s0, r',o) then true else true;
-// assert eval_code(Block(lvm_b0), lvm_s0, lvm_s0,o);
-//   assert evalBlock(lvm_b0, lvm_s0, lvm_sN,o);
-  
-//   assert eval_code(Block(lvm_b0), lvm_s0, lvm_sN,o);
+
+  assert evalBlock(lvm_b0, lvm_s0, lvm_sN,o) ==> exists r' :: evalCode(lvm_b0.hd, lvm_s0, r',o) && evalBlock(lvm_b0.tl, r', lvm_sN,o);
+  assert exists r' :: if evalCode(lvm_b0.hd, lvm_s0, r',o) then true else true;
+
+
   ghost var lvm_ltmp1, lvm_cM:lvm_code, lvm_ltmp2 := lvm_lemma_block_lax(lvm_b0, lvm_s0, lvm_sN,o);
   lvm_sM := lvm_ltmp1;
   lvm_bM := lvm_ltmp2;
@@ -55,50 +52,46 @@ assert exists r' :: if evalCode(lvm_b0.hd, lvm_s0, r',o) then true else true;
 ////
     // test(src){
     //     src = src + 4;
-    //     return void
     // }
 ///
-function method{:opaque} lvm_code_Add(dst:lvm_operand_opr, size:nat, src1:lvm_operand_opr):lvm_code
+function method{:opaque} lvm_code_Add_single(dst:lvm_operand_opr, size:nat, src1:lvm_operand_opr):lvm_code
 {
     reveal_IntFits();
     var val := D(Int(4,IntType(1,false)));
     assert val.d.Int?;
     var void := D(Void);
-    lvm_Block(lvm_CCons(Ins(ADD(dst, size,src1,val)),lvm_CCons(Ins(RET(void)),lvm_CNil())))
+    lvm_Block(lvm_CCons(Ins(ADD(dst, size,src1,val)),lvm_CNil()))
+
+    // lvm_Block(lvm_CCons(Ins(ADD(dst, size,src1,val)),lvm_CCons(Ins(RET(void)),lvm_CNil())))
 
 }
 
-lemma lvm_lemma_Add(lvm_b0:lvm_codes, lvm_s0:lvm_state, lvm_sN:lvm_state, 
+lemma lvm_lemma_Add_single(lvm_b0:lvm_codes, lvm_s0:lvm_state, lvm_sN:lvm_state, 
             dst:lvm_operand_opr, size:nat, src1:lvm_operand_opr,src2:lvm_operand_opr,o:operand)
   returns (lvm_bM:lvm_codes, lvm_sM:lvm_state)
-  requires lvm_require(lvm_b0, lvm_code_Add(dst, size,src1), lvm_s0, lvm_sN,dst)
+  requires lvm_require(lvm_b0, lvm_code_Add_single(dst, size,src1), lvm_s0, lvm_sN,dst)
   requires lvm_is_dst_opr(dst, lvm_s0)
   requires lvm_is_src_opr(src1, lvm_s0)
   requires lvm_get_ok(lvm_s0)
 
   requires ValidOperand(lvm_s0,src1);
   requires OperandContents(lvm_s0,src1).Int?;
-  requires lvm_code_Add(dst, size,src1).Ins?;
-
-//   requires dst.GV?;
+  requires lvm_code_Add_single(dst, size,src1).Ins?;
   requires ValidOperand(lvm_s0,dst)
 //   
   ensures  lvm_ensure(lvm_b0, lvm_bM, lvm_s0, lvm_sM, lvm_sN,dst)
   ensures  lvm_get_ok(lvm_sM)
   ensures ValidOperand(lvm_sM,dst)
-
   ensures OperandContents(lvm_sM,dst).Int?;
   ensures OperandContents(lvm_s0,dst).Int?;
-
   ensures  OperandContents(lvm_sM, dst).val == OperandContents(lvm_s0, dst).val + 4
   ensures  lvm_state_eq(lvm_sM, lvm_update_ok(lvm_sM, lvm_update_mem( lvm_sM, lvm_s0)))
 {
-    // assert dst.g in lvm_s0.gvs;
-  reveal_lvm_code_Add();
-  assert lvm_code_Add(dst, size,src1).Ins?;
-  var addIns := lvm_code_Add(dst, size,src1).ins;
+  reveal_lvm_code_Add_single();
+  assert lvm_code_Add_single(dst, size,src1).Ins?;
+  var addIns := lvm_code_Add_single(dst, size,src1).ins;
   assert ValidInstruction(lvm_s0,addIns);
-//   assert o == dst;
+
   assert  ValidRegOperand(lvm_s0, dst);
   assert ValidState(lvm_s0);
   assert lvm_b0.hd.Ins?;
@@ -113,10 +106,158 @@ lemma lvm_lemma_Add(lvm_b0:lvm_codes, lvm_s0:lvm_state, lvm_sN:lvm_state,
 
   assert evalCode_lax(lvm_cM, lvm_s0, lvm_sM,dst);
   assert OperandContents(lvm_sM, dst).val == OperandContents(lvm_s0, dst).val + 4;
-//   assert ValidInstruction(lvm_s0,lvm_code_Add(dst, size,src1,src2).ins) ==> lvm_sM.ok;
+
+  reveal_evalCodeOpaque();
+}
+
+
+///
+function method lvm_code_Add_Multiple(lvm_s0:lvm_state,dst:lvm_operand_opr, size:nat, src1:lvm_operand_opr): (out:lvm_code)
+    ensures out.Block?;
+    ensures out.block.lvm_CCons?;
+    ensures out.block.hd.Ins?;
+    // ensures out.hd.Ins?;
+    // ensures ValidInstruction(lvm_s0,out.block.hd.ins);
+{
+    reveal_IntFits();
+    var val := D(Int(4,IntType(1,false)));
+    assert val.d.Int?;
+    var void := D(Void);
+
+    var val2 := D(Int(5,IntType(1,false)));
+    assert val.d.Int?;
+
+    lvm_Block(lvm_CCons(Ins(ADD(dst,size,src1,val)),
+              lvm_CCons(Ins(ADD(dst,size,src1,val2)),lvm_CNil())))
+
+}
+
+lemma lvm_lemma_Add_Multiple(lvm_b0:lvm_codes, lvm_s0:lvm_state, lvm_sN:lvm_state, 
+            dst:lvm_operand_opr, size:nat, src1:lvm_operand_opr,src2:lvm_operand_opr,o:operand)
+  returns (lvm_bM:lvm_codes, lvm_sM:lvm_state)
+  requires lvm_require(lvm_b0, lvm_code_Add_Multiple(lvm_s0,dst, size,src1).block.hd, lvm_s0, lvm_sN,dst)
+  requires lvm_is_dst_opr(dst, lvm_s0)
+  requires lvm_is_src_opr(src1, lvm_s0)
+  requires lvm_get_ok(lvm_s0)
+
+  requires ValidOperand(lvm_s0,src1);
+  requires OperandContents(lvm_s0,src1).Int?;
+  requires ValidOperand(lvm_s0,dst);
+  requires ValidInstruction(lvm_s0,lvm_code_Add_Multiple(lvm_s0,dst, size,src1).block.hd.ins);
+//   requires lvm_code_Add_Multiple(lvm_s0,dst, size,src1).Ins?; //  ISSUE <<---
+
+  requires ValidOperand(lvm_s0,dst)
+//   
+  ensures  lvm_ensure(lvm_b0, lvm_bM, lvm_s0, lvm_sM, lvm_sN,dst)
+  ensures  lvm_get_ok(lvm_sM) 
+  ensures ValidOperand(lvm_sM,dst)
+
+  ensures OperandContents(lvm_sM,dst).Int?;
+  ensures OperandContents(lvm_s0,dst).Int?;
+
+  ensures  OperandContents(lvm_sM, dst).val == OperandContents(lvm_s0, dst).val + 9
+  ensures  lvm_state_eq(lvm_sM, lvm_update_ok(lvm_sM, lvm_update_mem( lvm_sM, lvm_s0)))
+{
+//   reveal_lvm_code_Add_Multiple();
+  assert lvm_code_Add_Multiple(lvm_s0,dst, size,src1).block.hd.Ins?;
+  var addIns := lvm_code_Add_Multiple(lvm_s0,dst, size,src1).block.hd.ins;
+
+  assert ValidInstruction(lvm_s0,addIns);
+  assert  ValidRegOperand(lvm_s0, dst);
+  assert ValidState(lvm_s0);
+//   assert lvm_b0.block.hd.Ins?;
+  var lvm_old_s:lvm_state := lvm_s0;
+//   lvm_ins_lemma(Ins(InsAdd(dst, src)), lvm_s0);
+  ghost var lvm_ltmp1, lvm_cM:lvm_code, lvm_ltmp2 := lvm_lemma_block(lvm_b0, lvm_s0, lvm_sN,dst);
+  lvm_sM := lvm_ltmp1;
+  lvm_bM := lvm_ltmp2;
+  assert lvm_b0.tl == lvm_bM;
+//   assert lvm_bM.CNil?;
+//   assert  OperandContents(lvm_sM, dst).Int?;
+
+  assert evalCode_lax(lvm_cM, lvm_s0, lvm_sM,dst);
+  assert OperandContents(lvm_sM, dst).val == OperandContents(lvm_s0, dst).val + 4;
+//   assert ValidInstruction(lvm_s0,lvm_code_Add_Multiple(dst, size,src1,src2).ins) ==> lvm_sM.ok;
 //   assert evalUpdate(lvm_s0, o, evalADD(size,OperandContents(lvm_s0,src1),val), lvm_sM);
 
   reveal_evalCodeOpaque();
 }
+
+
+
+// function method{:opaque} lvm_code_Add(dst:lvm_operand_opr, size:nat, src1:lvm_operand_opr): (out:lvm_code)
+//     ensures out.Block?;
+//     ensures out.block.lvm_CCons?;
+//     ensures out.block.hd.Ins?;
+// {
+//     reveal_IntFits();
+//     var val := D(Int(4,IntType(1,false)));
+//     assert val.d.Int?;
+//     var void := D(Void);
+//     lvm_Block(lvm_CCons(Ins(ADD(dst, size,src1,val)),lvm_CCons(Ins(RET(void)),lvm_CNil())))
+
+// }
+
+// lemma lvm_lemma_Add(lvm_b0:lvm_codes, lvm_s0:lvm_state, lvm_sN:lvm_state, 
+//             dst:lvm_operand_opr, size:nat, src1:lvm_operand_opr,src2:lvm_operand_opr,o:operand)
+//   returns (lvm_bM:lvm_codes, lvm_sM:lvm_state)
+//   requires lvm_require(lvm_b0, lvm_code_Add(dst, size,src1), lvm_s0, lvm_sN,dst)
+//   requires lvm_is_dst_opr(dst, lvm_s0)
+//   requires lvm_is_src_opr(src1, lvm_s0)
+//   requires lvm_get_ok(lvm_s0)
+
+//   requires ValidOperand(lvm_s0,src1);
+//   requires OperandContents(lvm_s0,src1).Int?;
+//   requires ValidInstruction(lvm_s0,lvm_code_Add(dst, size,src1).block.hd.ins);
+// //   requires lvm_code_Add(dst, size,src1).Ins?;
+
+// //   requires dst.GV?;
+//   requires ValidOperand(lvm_s0,dst)
+// //   
+//   ensures  lvm_ensure(lvm_b0, lvm_bM, lvm_s0, lvm_sM, lvm_sN,dst)
+//   ensures  lvm_get_ok(lvm_sM)
+//   ensures ValidOperand(lvm_sM,dst)
+
+//   ensures OperandContents(lvm_sM,dst).Int?;
+//   ensures OperandContents(lvm_s0,dst).Int?;
+
+//   ensures  OperandContents(lvm_sM, dst).val == OperandContents(lvm_s0, dst).val + 4
+//   ensures  lvm_state_eq(lvm_sM, lvm_update_ok(lvm_sM, lvm_update_mem( lvm_sM, lvm_s0)))
+// {
+//     // assert dst.g in lvm_s0.gvs;
+//   reveal_lvm_code_Add();
+//   assert lvm_code_Add(dst, size,src1).Block?;
+//   var addIns := lvm_code_Add(dst, size,src1).block.hd.ins;
+//   assert ValidInstruction(lvm_s0,addIns);
+// //   assert o == dst;
+//   assert  ValidRegOperand(lvm_s0, dst);
+//   assert ValidOperand(lvm_s0,dst);
+//   assert ValidState(lvm_s0);
+//   assert lvm_b0.hd.Block?;
+//   assert lvm_b0.hd == lvm_code_Add(dst, size,src1);
+// //   assert lvm_b0.hd.Ins?;
+//   var lvm_old_s:lvm_state := lvm_s0;
+// //   lvm_ins_lemma(Ins(InsAdd(dst, src)), lvm_s0);
+//   ghost var lvm_ltmp1, lvm_cM:lvm_code, lvm_ltmp2 := lvm_lemma_block_lax(lvm_b0, lvm_s0, lvm_sN,dst);
+//   lvm_sM := lvm_ltmp1;
+//   lvm_bM := lvm_ltmp2;
+//   assert lvm_b0.tl == lvm_bM;
+//   assert lvm_cM == lvm_b0.hd;
+// //   assert lvm_bM.CNil?;
+// //   assert  OperandContents(lvm_sM, dst).Int?;
+
+//   assert evalCode_lax(lvm_cM, lvm_s0, lvm_sM,dst);
+//   assert lvm_s0.ok;
+//   assert lvm_cM.block.hd.Ins?;
+//   assert exists r' :: evalCode(lvm_cM.block.hd,lvm_s0,r',dst);
+//   assert evalBlock(lvm_cM.block,lvm_s0, lvm_sM,dst);
+
+//   assert OperandContents(lvm_sM, dst).val == OperandContents(lvm_s0, dst).val + 4;
+// //   assert ValidInstruction(lvm_s0,lvm_code_Add(dst, size,src1,src2).ins) ==> lvm_sM.ok;
+// //   assert evalUpdate(lvm_s0, o, evalADD(size,OperandContents(lvm_s0,src1),val), lvm_sM);
+
+//   reveal_evalCodeOpaque();
+// }
+
 
 }
